RUBRIC.md
@@ -1,0 +1,26 @@
+Every algorithm or data structure should be formalized in the following structure:
+
+* CLRS.ChXX.AlgoName.Spec.fst
+    - Pure F* specification of the algorithm
+
+* CLRS.ChXX.AlgoName.Lemmas.fst
+    - Proofs of lemmas about the pure specification, e.g., optimiality results,
+      correctness properties of the spec etc.
+
+* CLRS.ChXX.AlgoName.Lemmas.fsti
+    - Interface file with signatures of the lemmas
+
+* CLRS.ChXX.AlgoName.Complexity.fst
+    - Proofs of the associated math lemmas about complexity properties, if any,
+      about the algorithm
+
+* CLRS.ChXX.AlgoName.Complexity.fsti
+    - Interface file with signatures of the complexity lemmas and any associated
+      definitions
+
+* CLRS.ChXX.AlgoName.Impl.fst
+    - Implementation of the algorithm in Pulse, proven to be functionally
+      equivalent to the specification as defined in AlgoName.Spec.fst
+
+* CLRS.ChXX.AlgoName.Impl.fsti
+    - Main public signature for the imperative implementation
